isabelle.sh
@@ -5,11 +5,13 @@ set -e
 DIR="$(dirname "$BASH_SOURCE[0]")"
 
 if [ "$#" = 0 ]; then
-    FILES=("$DIR/Quantum.thy")
+    FILES=("$DIR/Quantum2.thy")
 else
     FILES=()
 fi
 
+SESSION=Bounded_Operators-Prerequisites
+
 ISABELLE_DIR=/opt/Isabelle2021
 
-"$ISABELLE_DIR/bin/isabelle" jedit -l Bounded_Operators -d . "$ISABELLE_DIR/src/Pure/ROOT.ML" "${FILES[@]}" "$@" &
+"$ISABELLE_DIR/bin/isabelle" jedit -l "$SESSION" -d . "$ISABELLE_DIR/src/Pure/ROOT.ML" "${FILES[@]}" "$@" &
